Vizing/InversionGuarantee.lean
@@ -8,29 +8,129 @@ open Aux Graph EdgeColoring Fan Path
 
 variable
   {n c : Nat} {G : Graph n} (C : EdgeColoring c G)
-  {x y : Vertex n} {a b : Color c}
+  {x y : Vertex n} {a b : Color c} (ha : a.isSome)
 
 -- Maximality : all free colors on last vertex of fan are free on x
 
+include ha in
 theorem inversion_guarantee (F : Fan C x y)
   {C' : EdgeColoring c G}
   {P : Path C a b x}
-  (hC' : isInverted C C' P) :
+  (hC' : isInverted C C' P)
+  (ha1 : a ∈ freeColorsOn C (last F))
+  (hF : isMaximal F)
+  (hxy : color C (x, y) = none) :
   ∃ i : Fin F.val.size, a ∈ freeColorsOn C' F.val[i] := by
   by_cases h : ∃ j : Fin F.val.size, color C (x, F.val[j]) = a
   rcases h with ⟨j, hj⟩
-  have : j.val > 0 := by
+  have aux0 : j.val > 0 := by
     by_contra hc
     simp at hc
-    simp [hc, F.firstElemAx] at hj
-    sorry
-  sorry
-  have aux1 : a ∈ freeColorsOn C x := by sorry
-  have aux2 : P.val = [x] := by sorry
-  have aux3 : C' = C := by sorry
-  rw [aux3]
+    simp_all [F.firstElemAx, Option.isSome_iff_ne_none]
+  have aux1 : a ∈ freeColorsOn C F.val[j.val - 1] := by
+    rw [← hj]
+    have := F.colorAx
+    apply chain'_rel_of_idx_consec (Nat.sub_lt_of_lt j.isLt) (j.isLt) F.colorAx
+    omega
+  by_cases hp : F.val[j.val - 1] ∈ P.val
+  · use ⟨F.val.size - 1, (by simp; apply Array.size_pos_iff.mpr; exact F.nonemptyAx)⟩
+    apply freeColor_of_not_exists_and_isSome _ ha
+    simp [isInverted, isInverted_notmem, isInverted_mem, aux1, pathEdges, color] at hC'
+    rcases hC' with ⟨hC', _⟩
+    have ha2 := not_exists_of_freeColor C ha1
+    contrapose! ha2
+    rcases ha2 with ⟨v, hv⟩
+    use v
+    rw [← hv]
+    simp [color, last, Array.back_eq_getElem]
+    apply hC'
+    · rw [← mem_edgeSet_iff_present]
+      apply C'.representsEdgesAx
+      simp [color] at ⊢ hv
+      rwa [hv]
+    · by_contra hc
+      simp [last, Array.back] at ha1
+      simp [isMaximal] at hF
+      apply mem_pathEdges_if at hc
+      simp at hc
+      have : F.val[F.val.size - 1] ≠ F.val[j.val - 1] := by
+        by_contra hc
+        apply (List.Nodup.getElem_inj_iff F.nodupAx).mp at hc
+        have : j = F.val.size := by omega
+        have := j.isLt
+        omega
+      have := isLast_if C hp aux1
+      have := isLast_if C hc.left ha1
+      simp_all
+  · use ⟨j.val - 1, Nat.sub_lt_of_lt j.isLt⟩
+    apply freeColor_of_not_exists_and_isSome _ ha
+    apply not_exists_of_freeColor at aux1
+    contrapose! aux1
+    rcases aux1 with ⟨v, hv⟩
+    use v
+    rw [← hv]
+    simp [isInverted, isInverted_notmem] at hC'
+    rcases hC' with ⟨hC', _⟩
+    apply hC'
+    · rw [← mem_edgeSet_iff_present]
+      apply C'.representsEdgesAx
+      simp [color] at ⊢ hv
+      rwa [hv]
+    · apply not_mem_pathEdges_if
+      left
+      trivial
+  have aux0 : a ∈ freeColorsOn C x := by
+    simp [isMaximal] at hF
+    by_contra hc
+    simp [freeColorsOn, mem_allColors_if_isSome ha, incidentColorsOn] at hc
+    rcases Array.getElem_of_mem hc.left with ⟨i, hi1, hi2⟩
+    specialize hF ⟨i, (by rwa [← Fin.getElem_fin, C.sizeAx2] at hi1)⟩
+    apply hF ?_ ?_ (by simpa [color, hi2])
+    have := C.representsEdgesAx (x, ⟨i, (by rwa [← Fin.getElem_fin, C.sizeAx2] at hi1)⟩)
+    simp [hi2, ha, present] at this
+    apply (List.mem_erase_of_ne ?_).mpr
+    · tauto
+    · by_contra hc
+      subst hc
+      simp_all [color, Option.isSome_iff_ne_none]
+    · contrapose! h
+      simp [color]
+      rw [← hi2]
+      rcases Array.mem_iff_getElem.mp h with ⟨j, hj1, hj2⟩
+      apply Fin.exists_iff.mpr
+      use j, hj1
+      simp [hj2]
+  have aux1 : P.val = [x] := by
+    have h1 := P.nonemptyAx
+    have h2 := P.colorAx
+    have h3 := P.firstElemAx
+    rw [alternatesColor, alternates.eq_def] at h2
+    split at h2
+    · contradiction
+    · simp_all
+    · rename_i _ v₁ v₂ vs heq
+      have : v₂.val < (C.val[↑x]'(by rw [C.sizeAx1]; exact x.isLt)).size := by
+        rw [C.sizeAx2]
+        exact v₂.isLt
+      have : a ∈ C.val[x]'(by rw [C.sizeAx1]; exact x.isLt) := by
+        apply Array.mem_iff_getElem.mpr
+        use v₂
+        simp_all [color]
+      simp_all [color, freeColorsOn, incidentColorsOn, Option.isSome_iff_ne_none]
   use ⟨F.val.size - 1, (by simp; apply Array.size_pos_iff.mpr; exact F.nonemptyAx)⟩
-  sorry
+  apply freeColor_of_not_exists_and_isSome _ ha
+  simp [isInverted, isInverted_notmem, isInverted_mem, aux1, pathEdges, color] at hC'
+  apply not_exists_of_freeColor at ha1
+  contrapose! ha1
+  rcases ha1 with ⟨v, hv⟩
+  use v
+  rw [← hv]
+  simp [color, last, Array.back_eq_getElem]
+  apply hC'
+  rw [← mem_edgeSet_iff_present]
+  apply C'.representsEdgesAx
+  simp [color] at ⊢ hv
+  rwa [hv]
 
 def findSubfanWithColor (F : Fan C x y)
   (C' : EdgeColoring c G)
